tla-tree/ImmutableDiskTreeRefinement.dfy
@@ -8,6 +8,7 @@ import ImmutableDiskTreeImpl
 import opened ImmutableDiskTree
 import opened ImmutableDiskTreeInv
 import opened ImmutableDiskTreeHeight
+import opened ImmutableDiskTreeContent
 import opened ImmutableDiskTreeInterpretation
 import opened MissingLibrary
 import CrashableMap
@@ -24,6 +25,7 @@ predicate WFDiskState(k:Constants, s:Variables)
 
 function DiskView(k:Constants, s:Variables) : (diskView:View)
     requires WFDiskState(k, s)
+    ensures ImmutableDiskTreeImpl.FullView(k.impl, diskView)
 {
     ImmutableDiskTreeImpl.ViewOfDisk(s.disk.sectors)
 }
@@ -31,7 +33,9 @@ function DiskView(k:Constants, s:Variables) : (diskView:View)
 predicate SysInv(k:Constants, s:Variables)
 {
     && WFDiskState(k, s)
-    && TreeInv(k.impl, s.impl, DiskView(k, s))
+    && TreeInv(k.impl, s.impl, DiskView(k, s))  // TODO remove this dependency until GC time
+    && CacheLbasFitOnDisk(k.impl, s.impl)
+    && OneDatumPerKeyInv(LookupView(k.impl, s.impl.ephemeralTable, ViewThroughCache(k.impl, s.impl, DiskView(k, s))))
 }
 
 // I rewritten from ImmutableDiskTree namespace.
@@ -51,12 +55,10 @@ lemma InvImpliesRefinementInit(k:Constants, s:Variables)
     requires SysInv(k, s)
     ensures CrashableMap.Init(Jk(k), J(k, s))
 {
-    reveal_ISubtreePrefixView();
-    reveal_ISlotView();
-    var tv := PersistentTreeView(k.impl, DiskView(k, s));
-
-    assert ISubtreeView(tv, ROOT_ADDR()) == ISubtreePrefixView(tv, ROOT_ADDR(), /*slotCount*/ 1); // OBSERVE
-    assert IPersistentView(k.impl, DiskView(k, s)) == CrashableMap.EmptyMap(); // OBSERVE
+    reveal_AllValueLookups();
+    reveal_AllKeys();
+    reveal_ReachableValues();
+    assert ILookupView(PersistentLookupView(k.impl, DiskView(k, s))) == CrashableMap.EmptyMap();    // OBSERVE
 }
 
 function FetchStep(k:Constants, s:Variables, s':Variables) : (step:Step)
@@ -66,6 +68,36 @@ function FetchStep(k:Constants, s:Variables, s':Variables) : (step:Step)
     reveal_Next();
     var step :| NextStep(k, s, s', step);
     step
+}
+
+//lemma ViewOfCacheImpliesInCache()
+    //requires 
+
+lemma ViewOfCacheNestsInViewThroughCache(k:Constants, s:Variables)
+    requires WFDiskState(k, s)
+    requires CacheLbasFitOnDisk(k.impl, s.impl)
+    ensures ViewsNest(k.impl,
+        ImmutableDiskTreeImpl.ViewOfCache(s.impl.cache),
+        ViewThroughCache(k.impl, s.impl, DiskView(k, s)))
+{
+    ImmutableDiskTreeImpl.reveal_ViewOfCache();
+    reveal_ViewThroughCache();
+    var cacheView := ImmutableDiskTreeImpl.ViewOfCache(s.impl.cache);   // OBSERVE trigger
+}
+
+lemma LemmaQueryNext(k:Constants, s:Variables, s':Variables, step:Step)
+    requires Next(k, s, s')
+    requires SysInv(k, s)
+    requires SysInv(k, s')
+    requires NextStep(k, s, s', step)
+    requires step.impl.QueryActionStep?
+    requires step.impl.datum.value != EmptyValue();
+    ensures CrashableMap.NextStep(Jk(k), J(k, s), J(k, s'), CrashableMap.QueryStep(step.impl.datum))
+{
+    reveal_AllValueLookups();
+    ViewOfCacheNestsInViewThroughCache(k, s);
+    reveal_AllKeys();
+    reveal_ReachableValues();
 }
 
 lemma InvImpliesRefinementNext(k:Constants, s:Variables, s':Variables)
@@ -83,46 +115,59 @@ lemma InvImpliesRefinementNext(k:Constants, s:Variables, s':Variables)
 
     match step.impl {
         case QueryActionStep(lookup, datum) => {
-            assert datum.value == IEphemeralView(k.impl, s.impl, DiskView(k, s))[datum.key];
-            assert CrashableMap.Query(Ik, Is, Is', datum);
-            assert CrashableMap.NextStep(Ik, Is, Is', CrashableMap.QueryStep(datum));
+            if (datum.value != EmptyValue()) {
+                LemmaQueryNext(k, s, s', step);
+            } else {
+                assume false;
+            }
         }
         case InsertActionStep(edit, datum) => {
+            assume false;
             assert CrashableMap.Write(Ik, Is, Is', datum);
             assert CrashableMap.NextStep(Ik, Is, Is', CrashableMap.WriteStep(datum));
         }
         case DeleteActionStep(edit, datum) => {
+            assume false;
             var emptyWrite := Datum(datum.key, EmptyValue());
             assert CrashableMap.Write(Ik, Is, Is', emptyWrite);
             assert CrashableMap.NextStep(Ik, Is, Is', CrashableMap.WriteStep(emptyWrite));
         }
         case ExpandActionStep(j) => {
+            assume false;
             assert CrashableMap.Stutter(Ik, Is, Is');
         }
         case ContractActionStep(j) => {
+            assume false;
             assert CrashableMap.Stutter(Ik, Is, Is');
         }
         case WriteBackActionStep(lba) => {
+            assume false;
             assert CrashableMap.Stutter(Ik, Is, Is');
             assert CrashableMap.NextStep(Ik, Is, Is', CrashableMap.StutterStep);
         }
         case EmitTableActionStep(persistentTi, super, tblSectorIdx) => {
+            assume false;
             assert CrashableMap.Stutter(Ik, Is, Is');
             assert CrashableMap.NextStep(Ik, Is, Is', CrashableMap.StutterStep);
         }
         case CommitActionStep(persistentTi, super) => {
+            assume false;
             assert CrashableMap.PersistWrites(Ik, Is, Is', 1);
         }
         case CrashActionStep => {
+            assume false;
             assert CrashableMap.SpontaneousCrash(Ik, Is, Is');
         }
         case RecoverActionStep(super, persistentTl) => {
+            assume false;
             assert CrashableMap.Stutter(Ik, Is, Is');
         }
         case CacheFaultActionStep(lba, sector) => {
+            assume false;
             assert CrashableMap.Stutter(Ik, Is, Is');
         }
         case CacheEvictActionStep(lba) => {
+            assume false;
             assert CrashableMap.Stutter(Ik, Is, Is');
         }
     }
